@prefix : <http://www.semanticweb.org/carlos/ontologies/2023/3/wines#> .
@prefix owl: <http://www.w3.org/2002/07/owl#> .
@prefix rdf: <http://www.w3.org/1999/02/22-rdf-syntax-ns#> .
@prefix xml: <http://www.w3.org/XML/1998/namespace> .
@prefix xsd: <http://www.w3.org/2001/XMLSchema#> .
@prefix rdfs: <http://www.w3.org/2000/01/rdf-schema#> .
@base <http://www.semanticweb.org/carlos/ontologies/2023/3/wines#> .

<http://www.semanticweb.org/carlos/ontologies/2023/3/wines> rdf:type owl:Ontology ;
                                                             rdfs:comment "This is an ontology about wines from Spain created by Carlos and Guillem" .

#################################################################
#    Annotation properties
#################################################################

###  http://swrl.stanford.edu/ontologies/3.3/swrla.owl#isRuleEnabled
<http://swrl.stanford.edu/ontologies/3.3/swrla.owl#isRuleEnabled> rdf:type owl:AnnotationProperty .


###  http://www.w3.org/2000/01/rdf-schema#sameAs
rdfs:sameAs rdf:type owl:AnnotationProperty .


#################################################################
#    Object Properties
#################################################################

###  http://www.semanticweb.org/carlos/ontologies/2023/3/wines#hasCharacteristic
:hasCharacteristic rdf:type owl:ObjectProperty ;
                   rdfs:subPropertyOf owl:topObjectProperty ;
                   rdfs:domain :Wine ;
                   rdfs:range :Wine_Characteristics ;
                   rdfs:comment "This property links a wine to its various characteristics, such as alcohol content, acidity level, and body type. It has a one-to-many relationship, meaning that a wine can have many different characteristics, but each characteristic is associated with only one wine" .


###  http://www.semanticweb.org/carlos/ontologies/2023/3/wines#hasGrapeVariety
:hasGrapeVariety rdf:type owl:ObjectProperty ;
                 rdfs:subPropertyOf owl:topObjectProperty ;
                 rdfs:domain :Wine ;
                 rdfs:range :Grape_Variety ;
                 rdfs:comment "This property links a wine to its grapes variety, each grape is associated with only one wine" .


###  http://www.semanticweb.org/carlos/ontologies/2023/3/wines#hasMaduration
:hasMaduration rdf:type owl:ObjectProperty ;
               rdfs:subPropertyOf owl:topObjectProperty ;
               rdfs:domain :Wine ;
               rdfs:range :Aging ;
               rdfs:comment "This property links a wine to its maduration, each maduration is associated with only one wine" .


###  http://www.semanticweb.org/carlos/ontologies/2023/3/wines#hasRating
:hasRating rdf:type owl:ObjectProperty ;
           rdfs:subPropertyOf owl:topObjectProperty ;
           rdfs:domain :Wine ;
           rdfs:range :Wine_Rating ;
           rdfs:comment "This property links a wine to its rate score, each rate score is associated with only one wine" .


###  http://www.semanticweb.org/carlos/ontologies/2023/3/wines#isLocalProduct
:isLocalProduct rdf:type owl:ObjectProperty ;
                rdfs:subPropertyOf owl:topObjectProperty ;
                rdfs:domain :Wine ;
                rdfs:comment "The property determines if a wine is being sold at the same región where it's being produced." .


###  http://www.semanticweb.org/carlos/ontologies/2023/3/wines#locatedIn
:locatedIn rdf:type owl:ObjectProperty ;
           rdfs:subPropertyOf owl:topObjectProperty ;
           rdfs:domain :Winery ;
           rdfs:range :Region ;
           rdfs:comment "The property determines in which región is a winery located." .


###  http://www.semanticweb.org/carlos/ontologies/2023/3/wines#producedIn
:producedIn rdf:type owl:ObjectProperty ;
            rdfs:subPropertyOf owl:topObjectProperty ;
            rdfs:domain :Wine ;
            rdfs:range :Region ;
            rdfs:comment "This property links a wine to the wine region where it was produced. It has a one-to-many relationship, meaning that a wine region can have many different wines produced in it, but each wine is produced in only one region" .


###  http://www.semanticweb.org/carlos/ontologies/2023/3/wines#selledBy
:selledBy rdf:type owl:ObjectProperty ;
          rdfs:subPropertyOf owl:topObjectProperty ;
          rdfs:domain :Wine ;
          rdfs:range :Winery ;
          rdfs:comment "This property links a wine to the winery that selled it. It has a one-to-many relationship, meaning that a winery can sell many different wines, but each wine is selled by only one winery" .


#################################################################
#    Data properties
#################################################################

###  http://www.semanticweb.org/carlos/ontologies/2023/3/wines#acidityLevel
:acidityLevel rdf:type owl:DatatypeProperty ;
              rdfs:domain :Wine_Characteristics ;
              rdfs:range xsd:double ;
              rdfs:comment "This property specifies the acidity level of a wine. It has a data type of double" .


###  http://www.semanticweb.org/carlos/ontologies/2023/3/wines#alcoholContent
:alcoholContent rdf:type owl:DatatypeProperty ;
                rdfs:domain :Wine_Characteristics ;
                rdfs:range xsd:double ;
                rdfs:comment "This property specifies the alcohol content of a wine. It has a data type of double" .


###  http://www.semanticweb.org/carlos/ontologies/2023/3/wines#bodyType
:bodyType rdf:type owl:DatatypeProperty ;
          rdfs:domain :Wine_Characteristics ;
          rdfs:range xsd:string ;
          rdfs:comment "This property specifies the body type of a wine. It has a data type of string" .


###  http://www.semanticweb.org/carlos/ontologies/2023/3/wines#grapeVarietyName
:grapeVarietyName rdf:type owl:DatatypeProperty ;
                  rdfs:domain :Grape_Variety ;
                  rdfs:range xsd:string ;
                  rdfs:comment "This property specifies the name of a grape variety. It has a data type of string" .


###  http://www.semanticweb.org/carlos/ontologies/2023/3/wines#numberReviews
:numberReviews rdf:type owl:DatatypeProperty ;
               rdfs:domain :Wine ;
               rdfs:range xsd:integer ;
               rdfs:comment "This property specifies the number reviews of wine. It has a data type of integer" .


###  http://www.semanticweb.org/carlos/ontologies/2023/3/wines#wineMaduration
:wineMaduration rdf:type owl:DatatypeProperty ;
                rdfs:domain :Aging ;
                rdfs:range xsd:integer ;
                rdfs:comment "This property specifies the maduration of a wine. It has a data type of integer" .


###  http://www.semanticweb.org/carlos/ontologies/2023/3/wines#wineName
:wineName rdf:type owl:DatatypeProperty ;
          rdfs:domain :Wine ;
          rdfs:range xsd:string ;
          rdfs:comment "This property specifies the name of a wine. It has a data type of string" .


###  http://www.semanticweb.org/carlos/ontologies/2023/3/wines#winePrice
:winePrice rdf:type owl:DatatypeProperty ;
           rdfs:domain :Wine ;
           rdfs:range xsd:decimal ;
           rdfs:comment "This property specifies the price of a wine. It has a data type of double" .


###  http://www.semanticweb.org/carlos/ontologies/2023/3/wines#wineRating
:wineRating rdf:type owl:DatatypeProperty ;
            rdfs:domain :Wine ;
            rdfs:range xsd:decimal ;
            rdfs:comment "This property specifies the score given to a wine in a wine tasting. It has a data type of double" .


###  http://www.semanticweb.org/carlos/ontologies/2023/3/wines#wineRegionName
:wineRegionName rdf:type owl:DatatypeProperty ;
                rdfs:domain :Region ;
                rdfs:range xsd:string ;
                rdfs:comment "This property specifies the name of a wine region. It has a data type of string" .


###  http://www.semanticweb.org/carlos/ontologies/2023/3/wines#wineryName
:wineryName rdf:type owl:DatatypeProperty ;
            rdfs:domain :Winery ;
            rdfs:range xsd:string ;
            rdfs:comment "This property specifies the name of a winery. It has a data type of string" .


#################################################################
#    Classes
#################################################################

###  http://www.semanticweb.org/carlos/ontologies/2023/3/wines#Aging
:Aging rdf:type owl:Class ;
       rdfs:subClassOf :Wine ;
       rdfs:comment "he process of aging wine in barrels or bottles to enhance its flavor and complexity" .


###  http://www.semanticweb.org/carlos/ontologies/2023/3/wines#Collaborator
:Collaborator rdf:type owl:Class ;
              rdfs:subClassOf :Person .


###  http://www.semanticweb.org/carlos/ontologies/2023/3/wines#Gold_metal
:Gold_metal rdf:type owl:Class ;
            rdfs:subClassOf :Wine_Rating ;
            owl:disjointWith :Normal_metal ;
            rdfs:comment "A gold metal ranking wine" .


###  http://www.semanticweb.org/carlos/ontologies/2023/3/wines#Grand_reserve
:Grand_reserve rdf:type owl:Class ;
               rdfs:subClassOf :Aging ;
               rdfs:comment "A designation for high-quality wines that have been aged for a longer period of time than other wines from the same producer" .


###  http://www.semanticweb.org/carlos/ontologies/2023/3/wines#Grape_Variety
:Grape_Variety rdf:type owl:Class ;
               rdfs:subClassOf :Wine ;
               rdfs:comment "A type of grape used to make wine" .


###  http://www.semanticweb.org/carlos/ontologies/2023/3/wines#Large_winery
:Large_winery rdf:type owl:Class ;
              rdfs:subClassOf :Winery ;
              owl:disjointWith :Small_winery ;
              rdfs:comment "A winery that sells a large volume of wine" .


###  http://www.semanticweb.org/carlos/ontologies/2023/3/wines#Local_grapes
:Local_grapes rdf:type owl:Class ;
              rdfs:subClassOf :Grape_Variety ;
              rdfs:comment "Grape varieties that are native to a particular wine region or country" .


###  http://www.semanticweb.org/carlos/ontologies/2023/3/wines#Main_wine_region
:Main_wine_region rdf:type owl:Class ;
                  rdfs:subClassOf :Region ;
                  owl:disjointWith :Sub_wine_region ;
                  rdfs:comment "A primary wine-producing region within a country" .


###  http://www.semanticweb.org/carlos/ontologies/2023/3/wines#Normal_metal
:Normal_metal rdf:type owl:Class ;
              rdfs:subClassOf :Wine_Rating ;
              rdfs:comment "A normal metal ranking wine" .


###  http://www.semanticweb.org/carlos/ontologies/2023/3/wines#Person
:Person rdf:type owl:Class ;
        rdfs:subClassOf :Winery .


###  http://www.semanticweb.org/carlos/ontologies/2023/3/wines#Propietary
:Propietary rdf:type owl:Class ;
            rdfs:subClassOf :Person .


###  http://www.semanticweb.org/carlos/ontologies/2023/3/wines#Red_grapes
:Red_grapes rdf:type owl:Class ;
            rdfs:subClassOf :Grape_Variety ;
            rdfs:comment "Grape varieties used to produce red wine" .


###  http://www.semanticweb.org/carlos/ontologies/2023/3/wines#Red_wine
:Red_wine rdf:type owl:Class ;
          rdfs:subClassOf :Type_Wine ;
          rdfs:comment "Wine made from red or black grapes that have been fermented with the grape skins, giving it its characteristic color and tannins" .


###  http://www.semanticweb.org/carlos/ontologies/2023/3/wines#Region
:Region rdf:type owl:Class ;
        rdfs:subClassOf :Wine_location .


###  http://www.semanticweb.org/carlos/ontologies/2023/3/wines#Reserve
:Reserve rdf:type owl:Class ;
         rdfs:subClassOf :Aging ;
         rdfs:comment "A designation for wines that have been aged for a longer period of time than other wines from the same producer, but not as long as Grand Reserve wines" .


###  http://www.semanticweb.org/carlos/ontologies/2023/3/wines#Rose_wine
:Rose_wine rdf:type owl:Class ;
           rdfs:subClassOf :Type_Wine ;
           rdfs:comment "A type of wine that is pink in color and made from red grapes, but with a shorter period of skin contact than red wine, resulting in a lighter color and lower tannins" .


###  http://www.semanticweb.org/carlos/ontologies/2023/3/wines#Small_winery
:Small_winery rdf:type owl:Class ;
              rdfs:subClassOf :Winery ;
              rdfs:comment "A winery that sells a limited volume of wine" .


###  http://www.semanticweb.org/carlos/ontologies/2023/3/wines#Sub_wine_region
:Sub_wine_region rdf:type owl:Class ;
                 rdfs:subClassOf :Region ;
                 rdfs:comment "A smaller wine-producing region within a larger wine region, with distinct characteristics and regulations" .


###  http://www.semanticweb.org/carlos/ontologies/2023/3/wines#Type_Wine
:Type_Wine rdf:type owl:Class ;
           rdfs:subClassOf :Wine ;
           rdfs:comment "A broad categorization of wines based on their color and/or production method" .


###  http://www.semanticweb.org/carlos/ontologies/2023/3/wines#White_grapes
:White_grapes rdf:type owl:Class ;
              rdfs:subClassOf :Grape_Variety ;
              rdfs:comment "Grape varieties used to produce white wine" .


###  http://www.semanticweb.org/carlos/ontologies/2023/3/wines#White_wine
:White_wine rdf:type owl:Class ;
            rdfs:subClassOf :Type_Wine ;
            rdfs:comment "Wine made from white or green grapes that have been fermented without the grape skins, resulting in a lighter color and lower tannins than red wine" .


###  http://www.semanticweb.org/carlos/ontologies/2023/3/wines#Wine
:Wine rdf:type owl:Class ;
      rdfs:comment "A type of alcoholic beverage made from fermented grapes" .


###  http://www.semanticweb.org/carlos/ontologies/2023/3/wines#Wine_Characteristics
:Wine_Characteristics rdf:type owl:Class ;
                      rdfs:subClassOf :Wine ;
                      rdfs:comment "A particular trait or quality of a wine, such as its aroma or body" .


###  http://www.semanticweb.org/carlos/ontologies/2023/3/wines#Wine_Rating
:Wine_Rating rdf:type owl:Class ;
             rdfs:subClassOf :Wine ;
             rdfs:comment "A score or ranking assigned to a wine based on its quality or other characteristics" .


###  http://www.semanticweb.org/carlos/ontologies/2023/3/wines#Wine_location
:Wine_location rdf:type owl:Class ;
               rdfs:subClassOf :Wine ;
               rdfs:comment "A geographic area where wine grapes are grown and wine is produced" .


###  http://www.semanticweb.org/carlos/ontologies/2023/3/wines#Winery
:Winery rdf:type owl:Class ;
        rdfs:comment "A place where wine is selled" .


###  http://www.semanticweb.org/carlos/ontologies/2023/3/wines#Young_wine
:Young_wine rdf:type owl:Class ;
            rdfs:subClassOf :Aging ;
            rdfs:comment "A wine that has not been aged for an extended period of time and is meant to be consumed soon after bottling" .


#################################################################
#    Individuals
#################################################################

###  http://www.semanticweb.org/carlos/ontologies/2023/3/wines#Aglianico
:Aglianico rdf:type owl:NamedIndividual ,
                    :Red_grapes ;
           rdfs:sameAs "https://dbpedia.org/page/Aglianico" .


###  http://www.semanticweb.org/carlos/ontologies/2023/3/wines#Bodegas_Mauro
:Bodegas_Mauro rdf:type owl:NamedIndividual ,
                        :Small_winery ;
               :locatedIn :Castilla_y_Leon .


###  http://www.semanticweb.org/carlos/ontologies/2023/3/wines#Castilla_y_Leon
:Castilla_y_Leon rdf:type owl:NamedIndividual ,
                          :Sub_wine_region .


###  http://www.semanticweb.org/carlos/ontologies/2023/3/wines#Moscatel
:Moscatel rdf:type owl:NamedIndividual ,
                   :White_grapes ;
          rdfs:sameAs "https://dbpedia.org/page/Muscatel" .


###  http://www.semanticweb.org/carlos/ontologies/2023/3/wines#Ribera_del_Duero
:Ribera_del_Duero rdf:type owl:NamedIndividual ,
                           :Main_wine_region ;
                  rdfs:sameAs "https://dbpedia.org/page/Ribera_del_Duero" .


###  http://www.semanticweb.org/carlos/ontologies/2023/3/wines#Terreus_Paraje_de_Cueva_Baja
:Terreus_Paraje_de_Cueva_Baja rdf:type owl:NamedIndividual ,
                                       :Wine ;
                              :hasGrapeVariety :Moscatel ;
                              :producedIn :Castilla_y_Leon ;
                              :selledBy :Vega_Sicilia ;
                              :wineMaduration 30 ;
                              :winePrice 66.07 ;
                              :wineRating 70 .


###  http://www.semanticweb.org/carlos/ontologies/2023/3/wines#Unico
:Unico rdf:type owl:NamedIndividual ,
                :Wine ;
       :hasGrapeVariety :Aglianico ;
       :producedIn :Ribera_del_Duero ;
       :selledBy :Vega_Sicilia ;
       :wineMaduration 100 ;
       :winePrice 2087.25 ;
       :wineRating 4.7 .


###  http://www.semanticweb.org/carlos/ontologies/2023/3/wines#Vega_Sicilia
:Vega_Sicilia rdf:type owl:NamedIndividual ,
                       :Large_winery ;
              :locatedIn :Ribera_del_Duero .


#################################################################
#    General axioms
#################################################################

[ rdf:type owl:AllDisjointClasses ;
  owl:members ( :Grand_reserve
                :Reserve
                :Young_wine
              )
] .


[ rdf:type owl:AllDisjointClasses ;
  owl:members ( :Local_grapes
                :Red_grapes
                :White_grapes
              )
] .


[ rdf:type owl:AllDisjointClasses ;
  owl:members ( :Red_wine
                :Rose_wine
                :White_wine
              )
] .


#################################################################
#    Rules
#################################################################

<http://www.semanticweb.org/carlos/ontologies/2023/3/untitled-ontology-3/w> rdf:type <http://www.w3.org/2003/11/swrl#Variable> .

<http://www.semanticweb.org/carlos/ontologies/2023/3/untitled-ontology-3/s> rdf:type <http://www.w3.org/2003/11/swrl#Variable> .

<http://www.semanticweb.org/carlos/ontologies/2023/3/untitled-ontology-3/r> rdf:type <http://www.w3.org/2003/11/swrl#Variable> .

<urn:swrl:var#w> rdf:type <http://www.w3.org/2003/11/swrl#Variable> .

<urn:swrl:var#gv> rdf:type <http://www.w3.org/2003/11/swrl#Variable> .

<http://www.semanticweb.org/carlos/ontologies/2023/3/untitled-ontology-3/period> rdf:type <http://www.w3.org/2003/11/swrl#Variable> .

[ <http://swrl.stanford.edu/ontologies/3.3/swrla.owl#isRuleEnabled> "true"^^xsd:boolean ;
   rdfs:comment "Cheks if wine is a local product" ;
   rdfs:label "LocalProduct" ;
   rdf:type <http://www.w3.org/2003/11/swrl#Imp> ;
   <http://www.w3.org/2003/11/swrl#body> [ rdf:type <http://www.w3.org/2003/11/swrl#AtomList> ;
                                           rdf:first [ rdf:type <http://www.w3.org/2003/11/swrl#IndividualPropertyAtom> ;
                                                       <http://www.w3.org/2003/11/swrl#propertyPredicate> :selledBy ;
                                                       <http://www.w3.org/2003/11/swrl#argument1> <http://www.semanticweb.org/carlos/ontologies/2023/3/untitled-ontology-3/w> ;
                                                       <http://www.w3.org/2003/11/swrl#argument2> <http://www.semanticweb.org/carlos/ontologies/2023/3/untitled-ontology-3/s>
                                                     ] ;
                                           rdf:rest [ rdf:type <http://www.w3.org/2003/11/swrl#AtomList> ;
                                                      rdf:first [ rdf:type <http://www.w3.org/2003/11/swrl#IndividualPropertyAtom> ;
                                                                  <http://www.w3.org/2003/11/swrl#propertyPredicate> :locatedIn ;
                                                                  <http://www.w3.org/2003/11/swrl#argument1> <http://www.semanticweb.org/carlos/ontologies/2023/3/untitled-ontology-3/s> ;
                                                                  <http://www.w3.org/2003/11/swrl#argument2> <http://www.semanticweb.org/carlos/ontologies/2023/3/untitled-ontology-3/r>
                                                                ] ;
                                                      rdf:rest [ rdf:type <http://www.w3.org/2003/11/swrl#AtomList> ;
                                                                 rdf:first [ rdf:type <http://www.w3.org/2003/11/swrl#ClassAtom> ;
                                                                             <http://www.w3.org/2003/11/swrl#classPredicate> :Wine ;
                                                                             <http://www.w3.org/2003/11/swrl#argument1> <http://www.semanticweb.org/carlos/ontologies/2023/3/untitled-ontology-3/w>
                                                                           ] ;
                                                                 rdf:rest [ rdf:type <http://www.w3.org/2003/11/swrl#AtomList> ;
                                                                            rdf:first [ rdf:type <http://www.w3.org/2003/11/swrl#IndividualPropertyAtom> ;
                                                                                        <http://www.w3.org/2003/11/swrl#propertyPredicate> :producedIn ;
                                                                                        <http://www.w3.org/2003/11/swrl#argument1> <http://www.semanticweb.org/carlos/ontologies/2023/3/untitled-ontology-3/w> ;
                                                                                        <http://www.w3.org/2003/11/swrl#argument2> <http://www.semanticweb.org/carlos/ontologies/2023/3/untitled-ontology-3/r>
                                                                                      ] ;
                                                                            rdf:rest rdf:nil
                                                                          ]
                                                               ]
                                                    ]
                                         ] ;
   <http://www.w3.org/2003/11/swrl#head> [ rdf:type <http://www.w3.org/2003/11/swrl#AtomList> ;
                                           rdf:first [ rdf:type <http://www.w3.org/2003/11/swrl#IndividualPropertyAtom> ;
                                                       <http://www.w3.org/2003/11/swrl#propertyPredicate> :isLocalProduct ;
                                                       <http://www.w3.org/2003/11/swrl#argument1> <http://www.semanticweb.org/carlos/ontologies/2023/3/untitled-ontology-3/w> ;
                                                       <http://www.w3.org/2003/11/swrl#argument2> <http://www.semanticweb.org/carlos/ontologies/2023/3/untitled-ontology-3/r>
                                                     ] ;
                                           rdf:rest rdf:nil
                                         ]
 ] .

[ <http://swrl.stanford.edu/ontologies/3.3/swrla.owl#isRuleEnabled> "true"^^xsd:boolean ;
   rdfs:comment "Check if wine is white" ;
   rdfs:label "CheckWhiteWine" ;
   rdf:type <http://www.w3.org/2003/11/swrl#Imp> ;
   <http://www.w3.org/2003/11/swrl#body> [ rdf:type <http://www.w3.org/2003/11/swrl#AtomList> ;
                                           rdf:first [ rdf:type <http://www.w3.org/2003/11/swrl#IndividualPropertyAtom> ;
                                                       <http://www.w3.org/2003/11/swrl#propertyPredicate> :hasGrapeVariety ;
                                                       <http://www.w3.org/2003/11/swrl#argument1> <urn:swrl:var#w> ;
                                                       <http://www.w3.org/2003/11/swrl#argument2> <urn:swrl:var#gv>
                                                     ] ;
                                           rdf:rest [ rdf:type <http://www.w3.org/2003/11/swrl#AtomList> ;
                                                      rdf:first [ rdf:type <http://www.w3.org/2003/11/swrl#ClassAtom> ;
                                                                  <http://www.w3.org/2003/11/swrl#classPredicate> :White_grapes ;
                                                                  <http://www.w3.org/2003/11/swrl#argument1> <urn:swrl:var#gv>
                                                                ] ;
                                                      rdf:rest [ rdf:type <http://www.w3.org/2003/11/swrl#AtomList> ;
                                                                 rdf:first [ rdf:type <http://www.w3.org/2003/11/swrl#ClassAtom> ;
                                                                             <http://www.w3.org/2003/11/swrl#classPredicate> :Wine ;
                                                                             <http://www.w3.org/2003/11/swrl#argument1> <urn:swrl:var#w>
                                                                           ] ;
                                                                 rdf:rest rdf:nil
                                                               ]
                                                    ]
                                         ] ;
   <http://www.w3.org/2003/11/swrl#head> [ rdf:type <http://www.w3.org/2003/11/swrl#AtomList> ;
                                           rdf:first [ rdf:type <http://www.w3.org/2003/11/swrl#ClassAtom> ;
                                                       <http://www.w3.org/2003/11/swrl#classPredicate> :White_wine ;
                                                       <http://www.w3.org/2003/11/swrl#argument1> <urn:swrl:var#w>
                                                     ] ;
                                           rdf:rest rdf:nil
                                         ]
 ] .

[ rdf:type <http://www.w3.org/2003/11/swrl#Imp> ;
   <http://www.w3.org/2003/11/swrl#body> [ rdf:type <http://www.w3.org/2003/11/swrl#AtomList> ;
                                           rdf:first [ rdf:type <http://www.w3.org/2003/11/swrl#IndividualPropertyAtom> ;
                                                       <http://www.w3.org/2003/11/swrl#propertyPredicate> :hasGrapeVariety ;
                                                       <http://www.w3.org/2003/11/swrl#argument1> <urn:swrl:var#w> ;
                                                       <http://www.w3.org/2003/11/swrl#argument2> <urn:swrl:var#gv>
                                                     ] ;
                                           rdf:rest [ rdf:type <http://www.w3.org/2003/11/swrl#AtomList> ;
                                                      rdf:first [ rdf:type <http://www.w3.org/2003/11/swrl#ClassAtom> ;
                                                                  <http://www.w3.org/2003/11/swrl#classPredicate> :Wine ;
                                                                  <http://www.w3.org/2003/11/swrl#argument1> <urn:swrl:var#w>
                                                                ] ;
                                                      rdf:rest [ rdf:type <http://www.w3.org/2003/11/swrl#AtomList> ;
                                                                 rdf:first [ rdf:type <http://www.w3.org/2003/11/swrl#ClassAtom> ;
                                                                             <http://www.w3.org/2003/11/swrl#classPredicate> :Red_grapes ;
                                                                             <http://www.w3.org/2003/11/swrl#argument1> <urn:swrl:var#gv>
                                                                           ] ;
                                                                 rdf:rest rdf:nil
                                                               ]
                                                    ]
                                         ] ;
   <http://www.w3.org/2003/11/swrl#head> [ rdf:type <http://www.w3.org/2003/11/swrl#AtomList> ;
                                           rdf:first [ rdf:type <http://www.w3.org/2003/11/swrl#ClassAtom> ;
                                                       <http://www.w3.org/2003/11/swrl#classPredicate> :Red_wine ;
                                                       <http://www.w3.org/2003/11/swrl#argument1> <urn:swrl:var#w>
                                                     ] ;
                                           rdf:rest rdf:nil
                                         ]
 ] .

[ <http://swrl.stanford.edu/ontologies/3.3/swrla.owl#isRuleEnabled> "true"^^xsd:boolean ;
   rdfs:comment "Checks if wine is a grand reserve" ;
   rdfs:label "WineMaduration" ;
   rdf:type <http://www.w3.org/2003/11/swrl#Imp> ;
   <http://www.w3.org/2003/11/swrl#body> [ rdf:type <http://www.w3.org/2003/11/swrl#AtomList> ;
                                           rdf:first [ rdf:type <http://www.w3.org/2003/11/swrl#BuiltinAtom> ;
                                                       <http://www.w3.org/2003/11/swrl#builtin> <http://www.w3.org/2003/11/swrlb#greaterThan> ;
                                                       <http://www.w3.org/2003/11/swrl#arguments> [ rdf:type rdf:List ;
                                                                                                    rdf:first <http://www.semanticweb.org/carlos/ontologies/2023/3/untitled-ontology-3/period> ;
                                                                                                    rdf:rest [ rdf:type rdf:List ;
                                                                                                               rdf:first 29 ;
                                                                                                               rdf:rest rdf:nil
                                                                                                             ]
                                                                                                  ]
                                                     ] ;
                                           rdf:rest [ rdf:type <http://www.w3.org/2003/11/swrl#AtomList> ;
                                                      rdf:first [ rdf:type <http://www.w3.org/2003/11/swrl#ClassAtom> ;
                                                                  <http://www.w3.org/2003/11/swrl#classPredicate> :Wine ;
                                                                  <http://www.w3.org/2003/11/swrl#argument1> <http://www.semanticweb.org/carlos/ontologies/2023/3/untitled-ontology-3/w>
                                                                ] ;
                                                      rdf:rest [ rdf:type <http://www.w3.org/2003/11/swrl#AtomList> ;
                                                                 rdf:first [ rdf:type <http://www.w3.org/2003/11/swrl#DatavaluedPropertyAtom> ;
                                                                             <http://www.w3.org/2003/11/swrl#propertyPredicate> :wineMaduration ;
                                                                             <http://www.w3.org/2003/11/swrl#argument1> <http://www.semanticweb.org/carlos/ontologies/2023/3/untitled-ontology-3/w> ;
                                                                             <http://www.w3.org/2003/11/swrl#argument2> <http://www.semanticweb.org/carlos/ontologies/2023/3/untitled-ontology-3/period>
                                                                           ] ;
                                                                 rdf:rest rdf:nil
                                                               ]
                                                    ]
                                         ] ;
   <http://www.w3.org/2003/11/swrl#head> [ rdf:type <http://www.w3.org/2003/11/swrl#AtomList> ;
                                           rdf:first [ rdf:type <http://www.w3.org/2003/11/swrl#ClassAtom> ;
                                                       <http://www.w3.org/2003/11/swrl#classPredicate> :Grand_reserve ;
                                                       <http://www.w3.org/2003/11/swrl#argument1> <http://www.semanticweb.org/carlos/ontologies/2023/3/untitled-ontology-3/w>
                                                     ] ;
                                           rdf:rest rdf:nil
                                         ]
 ] .

###  Generated by the OWL API (version 5.1.18) https://github.com/owlcs/owlapi/
